Cleaning up code in ExpRel and STLC. Moved history independence stuff to old folder. Deleted unused definitions in IO.

rupicola/io/STLC.fst
@@ -611,17 +611,6 @@ let lem_irred_implies_srefl_steps (#e #e':closed_exp) (#h:history) (#lt:local_tr
   | SRefl e h -> ()
   | STrans _ _ -> false_elim ()
 
-let lem_value_preserves_value (e:closed_exp) (h:history) :
-  Lemma (requires is_value e)
-        (ensures (forall e' lt. steps e e' h lt /\ indexed_irred e' (h++lt) ==> is_value e')) =
-  introduce forall e' lt. steps e e' h lt /\ indexed_irred e' (h++lt) ==> is_value e' with begin
-    introduce _ ==> _ with _. begin
-      lem_value_is_irred e;
-      FStar.Squash.bind_squash #(steps e e' h lt) () (fun sts ->
-      lem_irred_implies_srefl_steps sts)
-    end
-  end
-
 let get_read_arg (ev:event{EvRead? ev}) : io_args ORead =
   match ev with
   | EvRead arg res -> arg
@@ -645,6 +634,14 @@ let get_einl_v (x:closed_exp{EInl? x}) =
 let get_einr_v (x:closed_exp{EInr? x}) =
   match x with
   | EInr v -> v
+
+let get_epair_e1 (x:closed_exp{EPair? x}) =
+  match x with
+  | EPair e1 e2 -> e1
+
+let get_epair_e2 (x:closed_exp{EPair? x}) =
+  match x with
+  | EPair e1 e2 -> e2
 
 //assume val get_new_file_descr (ev:event{EvOpen? ev}) (h':history) : (ev':event{test_event h' ev'})
 
@@ -708,16 +705,24 @@ let sem_value_shape (t:typ) (e:closed_exp) : Tot Type0 =
   match t with
   | TUnit -> e == EUnit
   | TBool -> e == ETrue \/ e == EFalse
-  | TArr t1 t2 -> ELam? e
-  | TPair t1 t2 -> EPair? e
   | TFileDescr -> EFileDescr? e
-  | TSum t1 t2 -> EInl? e \/ EInr? e
-
-let sem_expr_shape (t:typ) (e:closed_exp) : Tot Type0 =
-  forall (e':closed_exp) (h:history) (lt:local_trace h). steps e e' h lt ==> irred e' ==> sem_value_shape t e'
+  | TArr t1 t2 -> ELam? e /\ is_closed e
+  | TPair t1 t2 -> EPair? e /\ is_value (get_epair_e1 e) /\ is_value (get_epair_e2 e)
+  | TSum t1 t2 -> (EInl? e /\ is_value (get_einl_v e)) \/ (EInr? e /\ is_value (get_einr_v e))
 
 let indexed_sem_expr_shape (t:typ) (e:closed_exp) (h:history) : Tot Type0 =
-  forall (e':closed_exp) (lt:local_trace h). steps e e' h lt ==> indexed_irred e' (h++lt) ==> sem_value_shape t e'
+  forall (e':closed_exp) (lt:local_trace h). steps e e' h lt /\ indexed_irred e' (h++lt) ==> sem_value_shape t e'
+
+let lem_value_preserves_value (e:closed_exp) (h:history) (t:typ) :
+  Lemma (requires is_value e /\ sem_value_shape t e)
+        (ensures indexed_sem_expr_shape t e h) =
+  introduce forall e' lt. steps e e' h lt /\ indexed_irred e' (h++lt) ==> sem_value_shape t e' with begin 
+    introduce _ ==> _ with _. begin
+      lem_value_is_irred e;
+      FStar.Squash.bind_squash #(steps e e' h lt) () (fun sts ->
+      lem_irred_implies_srefl_steps sts)
+    end
+  end
 
 let lem_step_preserve_indexed_sem_expr_shape (e e':closed_exp) (h:history) (oev:option (event_h h)) (t:typ) :
   Lemma
@@ -726,98 +731,31 @@ let lem_step_preserve_indexed_sem_expr_shape (e e':closed_exp) (h:history) (oev:
   introduce forall e'' lt'. steps e' e'' (h++(as_lt oev)) lt' /\ indexed_irred e'' ((h++(as_lt oev))++lt') ==> sem_value_shape t e'' with begin
     introduce _  ==> sem_value_shape t e'' with _. begin
       lem_step_implies_steps e e' h oev;
-      lem_steps_transitive e e' e'' h (as_lt oev) lt';
-      eliminate forall e' lt. steps e e' h lt /\ indexed_irred e' (h++lt) ==> sem_value_shape t e' with e'' ((as_lt oev) @ lt');
-      ()
-    end
-  end
-
-let lem_steps_preserve_is_value (e e_ :closed_exp) (h:history) (lt_:local_trace h) :
-  Lemma (requires (forall e' lt. steps e e' h lt /\ indexed_irred e' (h++lt) ==> is_value e') /\ steps e e_ h lt_)
-        (ensures (forall e' lt. steps e_ e' (h++lt_) lt /\ indexed_irred e' ((h++lt_)++lt) ==> is_value e')) =
-  introduce forall e' lt. steps e_ e' (h++lt_) lt /\ indexed_irred e' ((h++lt_)++lt) ==> is_value e' with begin
-    introduce _ ==> _ with _. begin
-      lem_steps_transitive e e_ e' h lt_ lt
-    end
-  end
-
-let lem_steps_preserve_is_lam_value (e e_ :closed_exp) (h:history) (lt_:local_trace h) :
-  Lemma (requires (forall e' lt. steps e e' h lt /\ indexed_irred e' (h++lt) ==> (ELam? e' /\ is_closed e')) /\ steps e e_ h lt_)
-        (ensures (forall e' lt. steps e_ e' (h++lt_) lt /\ indexed_irred e' ((h++lt_)++lt) ==> (ELam? e' /\ is_closed e'))) =
-  introduce forall e' lt. steps e_ e' (h++lt_) lt /\ indexed_irred e' ((h++lt_)++lt) ==> (ELam? e' /\ is_closed e') with begin
-    introduce _ ==> _ with _. begin
-      lem_steps_transitive e e_ e' h lt_ lt
-    end
-  end
-
-let lem_steps_preserve_is_bool_value (e e_ :closed_exp) (h:history) (lt_:local_trace h) :
-  Lemma (requires (forall e' lt. steps e e' h lt /\ indexed_irred e' (h++lt) ==> (ETrue? e' \/ EFalse? e')) /\ steps e e_ h lt_)
-        (ensures (forall e' lt. steps e_ e' (h++lt_) lt /\ indexed_irred e' ((h++lt_)++lt) ==> (ETrue? e' \/ EFalse? e'))) =
-  introduce forall e' lt. steps e_ e' (h++lt_) lt /\ indexed_irred e' ((h++lt_)++lt) ==> (ETrue? e' \/ EFalse? e') with begin
-    introduce _ ==> _ with _. begin
-      lem_steps_transitive e e_ e' h lt_ lt
-    end
-  end
-
-let lem_steps_preserve_is_pair_value (e e_ :closed_exp) (h:history) (lt_:local_trace h) :
-  Lemma (requires (forall e' lt. steps e e' h lt /\ indexed_irred e' (h++lt) ==> (EPair? e' /\ is_value e')) /\ steps e e_ h lt_)
-        (ensures (forall e' lt. steps e_ e' (h++lt_) lt /\ indexed_irred e' ((h++lt_)++lt) ==> (EPair? e' /\ is_value e'))) =
-  introduce forall e' lt. steps e_ e' (h++lt_) lt /\ indexed_irred e' ((h++lt_)++lt) ==> (EPair? e' /\ is_value e') with begin
-    introduce _ ==> _ with _. begin
-      lem_steps_transitive e e_ e' h lt_ lt
-    end
-  end
-
-let lem_steps_preserve_is_sum_value (e e_ :closed_exp) (h:history) (lt_:local_trace h) :
-  Lemma (requires (forall e' lt. steps e e' h lt /\ indexed_irred e' (h++lt) ==> ((EInl? e' \/ EInr? e') /\ is_value e')) /\ steps e e_ h lt_)
-        (ensures (forall e' lt. steps e_ e' (h++lt_) lt /\ indexed_irred e' ((h++lt_)++lt) ==> ((EInl? e' \/ EInr? e') /\ is_value e'))) =
-  introduce forall e' lt. steps e_ e' (h++lt_) lt /\ indexed_irred e' ((h++lt_)++lt) ==> ((EInl? e' \/ EInr? e') /\ is_value e') with begin
-    introduce _ ==> _ with _. begin
-      lem_steps_transitive e e_ e' h lt_ lt
-    end
-  end
-
-let lem_steps_preserve_is_file_descr_value (e e_ :closed_exp) (h:history) (lt_:local_trace h) :
-  Lemma (requires (forall e' lt. steps e e' h lt /\ indexed_irred e' (h++lt) ==> (EFileDescr? e' /\ is_value e')) /\ steps e e_ h lt_)
-        (ensures (forall e' lt. steps e_ e' (h++lt_) lt /\ indexed_irred e' ((h++lt_)++lt) ==> (EFileDescr? e' /\ is_value e'))) =
-  introduce forall e' lt. steps e_ e' (h++lt_) lt /\ indexed_irred e' ((h++lt_)++lt) ==> (EFileDescr? e' /\ is_value e') with begin
-    introduce _ ==> _ with _. begin
-      lem_steps_transitive e e_ e' h lt_ lt
+      lem_steps_transitive e e' e'' h (as_lt oev) lt'
     end
   end
 
 // DESTRUCT LEMMAS
 
-let can_step_eapp_when_safe (e1 e2:closed_exp) (h:history) : Lemma
-  (requires
-    ((indexed_irred e1 h /\ steps e1 e1 h []) ==> (ELam? e1 /\ is_closed e1)) /\
-    ((indexed_irred e2 h /\ steps e2 e2 h []) ==> is_value e2))
+let can_step_eapp_when_reduced (e1:closed_exp) (e2:closed_exp{is_value e2}) (h:history) (t1 t2:typ) : Lemma
+  (requires indexed_sem_expr_shape (TArr t1 t2) e1 h)
   (ensures (exists e' oev. step (EApp e1 e2) e' h oev))
   =
   (**
      We case analyze if e1 can step or if e2 can step,
        and for each case, we build a step accordingly **)
 
-  introduce indexed_irred e1 h /\ indexed_irred e2 h ==> (exists e' oev. step (EApp e1 e2) e' h oev) with _. begin
+  introduce indexed_irred e1 h ==> (exists e' oev. step (EApp e1 e2) e' h oev) with _. begin
     assert (steps e1 e1 h []);
-    assert (steps e2 e2 h []);
     let ELam e11 = e1 in
     let st : step (EApp (ELam e11) e2) (subst_beta e2 e11) h None = Beta e11 e2 h in
     ()
   end;
 
-  introduce ~(indexed_irred e1 h) /\ indexed_irred e2 h ==> (exists e' oev. step (EApp e1 e2) e' h oev) with _. begin
-    assert (steps e2 e2 h []);
+  introduce ~(indexed_irred e1 h) ==> (exists e' oev. step (EApp e1 e2) e' h oev) with _. begin
     assert (exists e1' oev1. step e1 e1' h oev1);
     eliminate exists e1' oev1. step e1 e1' h oev1 returns exists e' oev. step (EApp e1 e2) e' h oev with st. begin
       bind_squash st (fun st -> return_squash (AppLeft e2 st))
-    end
-  end;
-
-  introduce ~(indexed_irred e2 h) ==>  (exists e' oev. step (EApp e1 e2) e' h oev) with _. begin
-    assert (exists e2' oev2. step e2 e2' h oev2);
-    eliminate exists e2' oev2. step e2 e2' h oev2 returns exists e' oev. step (EApp e1 e2) e' h oev with st. begin
-      bind_squash st (fun st -> return_squash (AppRight e1 st))
     end
   end
 
@@ -858,10 +796,11 @@ let rec destruct_steps_eapp_e1
   (e':closed_exp)
   (h:history)
   (lt:local_trace h)
-  (st:steps (EApp e1 e2') e' h lt) :
+  (st:steps (EApp e1 e2') e' h lt) 
+  (t1 t2:typ) :
   Pure (exp * (lt1:local_trace h & local_trace (h++lt1)))
     (requires indexed_irred e' (h++lt) /\
-              (forall e1' (lt1:local_trace h). (steps e1 e1' h lt1 /\ indexed_irred e1' (h++lt1)) ==> (ELam? e1' /\ is_closed e1')))
+      indexed_sem_expr_shape (TArr t1 t2) e1 h)
     (ensures fun (e11, (| lt1, lt' |)) ->
       is_closed (ELam e11) /\
       steps e1 (ELam e11) h lt1 /\
@@ -872,7 +811,7 @@ let rec destruct_steps_eapp_e1
     (decreases st) =
     match st with
     | SRefl (EApp e1 e2') h -> begin
-      can_step_eapp_when_safe e1 e2' h;
+      can_step_eapp_when_reduced e1 e2' h t1 t2;
       false_elim ()
       end
     | STrans #e #f2 #e' #h #_ #lt23 step_eapp step_eapp_steps -> begin
@@ -884,8 +823,8 @@ let rec destruct_steps_eapp_e1
         lem_step_implies_steps (EApp e1 e2') (EApp e1' e2') h oev1;
         let lt1 : local_trace h = as_lt oev1 in
         let s2 : steps (EApp e1' e2') e' (h++lt1) lt23 = step_eapp_steps in
-        lem_steps_preserve_is_lam_value e1 e1' h lt1;
-        let (e11, (| lt1', lt' |)) = destruct_steps_eapp_e1 e1' e2' e' (h++lt1) lt23 s2 in
+        lem_step_preserve_indexed_sem_expr_shape e1 e1' h oev1 (TArr t1 t2);
+        let (e11, (| lt1', lt' |)) = destruct_steps_eapp_e1 e1' e2' e' (h++lt1) lt23 s2 t1 t2 in
         lem_steps_transitive e1 e1' (ELam e11) h lt1 lt1';
         lem_steps_transitive (EApp e1 e2') (EApp e1' e2') (subst_beta e2' e11) h lt1 lt1';
         (e11, (| (lt1 @ lt1'), lt' |))
@@ -909,7 +848,7 @@ let rec destruct_steps_eapp_e2
   (st:steps (EApp e1 e2) e' h lt) :
   Pure (value * (lt2:local_trace h & local_trace (h++lt2)))
     (requires indexed_irred e' (h++lt) /\
-      (forall e2' lt2. steps e2 e2' h lt2 /\ indexed_irred e2' (h++lt2) ==> is_value e2'))
+      indexed_safe e2 h)
     (ensures fun (e2', (| lt2, lt' |)) ->
       steps e2 e2' h lt2 /\
       steps (EApp e1 e2) (EApp e1 e2') h lt2 /\
@@ -920,6 +859,7 @@ let rec destruct_steps_eapp_e2
     match st with
     | SRefl (EApp e1 e2) h -> begin
       lem_irred_eapp_implies_irred_e2 e1 e2 h;
+      assert (steps e2 e2 h []);
       (e2, (| [], lt |))
       end
     | STrans #e #f2 #e' #h #_ #lt23 step_eapp step_eapp_steps -> begin
@@ -931,7 +871,7 @@ let rec destruct_steps_eapp_e2
         lem_step_implies_steps (EApp e1 e2) (EApp e1 e2') h oev2;
         let lt2 : local_trace h = as_lt oev2 in
         let s2 : steps (EApp e1 e2') e' (h++lt2) lt23 = step_eapp_steps in
-        lem_steps_preserve_is_value e2 e2' h lt2;
+        lem_step_preserve_indexed_safe e2 e2' h oev2;
         let (e2'', (| lt2', lt' |)) = destruct_steps_eapp_e2 e1 e2' e' (h++lt2) lt23 s2 in
         lem_steps_transitive e2 e2' e2'' h lt2 lt2';
         lem_steps_transitive (EApp e1 e2) (EApp e1 e2') (EApp e1 e2'') h lt2 lt2';
@@ -941,8 +881,7 @@ let rec destruct_steps_eapp_e2
       end
 
 let can_step_eif_when_safe (e1 e2 e3:closed_exp) (h:history) : Lemma
-  (requires
-    (forall e1' lt1. (steps e1 e1' h lt1 /\ indexed_irred e1' (h++lt1)) ==> (ETrue? e1' \/ EFalse? e1')))
+  (requires indexed_sem_expr_shape TBool e1 h)
   (ensures (exists e' oev. step (EIf e1 e2 e3) e' h oev))
   =
   introduce indexed_irred e1 h /\ e1 == ETrue ==> (exists e' oev. step (EIf e1 e2 e3) e' h oev) with _. begin
@@ -979,7 +918,7 @@ let rec destruct_steps_eif
   (st:steps (EIf e1 e2 e3) e' h lt) :
   Pure (closed_exp * (lt1:local_trace h & (local_trace (h++lt1) * local_trace (h++lt1))))
     (requires indexed_irred e' (h++lt) /\
-       (forall e1' lt1. (steps e1 e1' h lt1 /\ indexed_irred e1' (h++lt1)) ==> (ETrue? e1' \/ EFalse? e1')))
+      indexed_sem_expr_shape TBool e1 h)
     (ensures fun (e1', (| lt1, (lt2, lt3) |)) ->
       indexed_irred e1' (h++lt1) /\
       steps e1 e1' h lt1 /\
@@ -1002,7 +941,7 @@ let rec destruct_steps_eif
         lem_step_implies_steps e1 e1' h oev1;
         lem_step_implies_steps (EIf e1 e2 e3) (EIf e1' e2 e3) h oev1;
         let lt1 : local_trace h = as_lt oev1 in
-        lem_steps_preserve_is_bool_value e1 e1' h lt1;
+        lem_step_preserve_indexed_sem_expr_shape e1 e1' h oev1 TBool;
         let s2 : steps (EIf e1' e2 e3) e' (h++lt1) lt23 = step_eif_steps in
         let (e1'', (| lt1', (lt2, lt3) |)) = destruct_steps_eif e1' e2 e3 e' (h++lt1) lt23 s2 in
         lem_steps_transitive e1 e1' e1'' h lt1 lt1';
@@ -1025,38 +964,6 @@ let rec destruct_steps_eif
     How the steps look like:
       EIf e1 e2 e3 -->* EIf e1' e2 e3 -->* e'
   **)
-
-let srefl_epair_implies_value (e1 e2:closed_exp) (h:history) : Lemma
-  (requires safe e1 /\ safe e2 /\ indexed_irred (EPair e1 e2) h)
-  (ensures is_value (EPair e1 e2))
-  =
-  introduce indexed_irred e1 h /\ indexed_irred e2 h ==> is_value (EPair e1 e2) with _.
-  begin
-    assert (steps e1 e1 h []);
-    assert (steps e2 e2 h []);
-    ()
-  end;
-
-  introduce ~(indexed_irred e1 h) ==> is_value (EPair e1 e2) with _.
-  begin
-    assert (exists e1' oev1. step e1 e1' h oev1);
-    eliminate exists e1' oev1. step e1 e1' h oev1 returns exists e' oev. step (EPair e1 e2) e' h oev with st.
-    begin
-      bind_squash st (fun st -> return_squash (PairLeft e2 st))
-    end;
-    false_elim ()
-  end;
-
-  introduce indexed_irred e1 h /\ ~(indexed_irred e2 h) ==> is_value (EPair e1 e2) with _.
-  begin
-    assert (steps e1 e1 h []);
-    assert (exists e2' oev2. step e2 e2' h oev2);
-    eliminate exists e2' oev2. step e2 e2' h oev2 returns exists e' oev. step (EPair e1 e2) e' h oev with st.
-    begin
-      bind_squash st (fun st -> return_squash (PairRight e1 st))
-    end;
-    false_elim ()
-  end
 
 let lem_irred_epair_implies_irred_e1 (e1 e2:closed_exp) (h:history) :
   Lemma (requires indexed_irred (EPair e1 e2) h)
@@ -1085,7 +992,7 @@ let rec destruct_steps_epair_e1
   (st:steps (EPair e1 e2) e' h lt) :
   Pure (value * (lt1:local_trace h & local_trace (h++lt1)))
     (requires indexed_irred e' (h++lt) /\
-      (forall e1' lt1. steps e1 e1' h lt1 /\ indexed_irred e1' (h++lt1) ==> is_value e1'))
+      indexed_safe e1 h)
     (ensures fun (e1', (| lt1, lt' |)) ->
       steps e1 e1' h lt1 /\
       steps (EPair e1 e2) (EPair e1' e2) h lt1 /\
@@ -1096,6 +1003,7 @@ let rec destruct_steps_epair_e1
   match st with
   | SRefl (EPair e1 e2) h -> begin
     lem_irred_epair_implies_irred_e1 e1 e2 h;
+    assert (steps e1 e1 h []);
     (e1, (| [], lt |))
     end
   | STrans #e #f2 #e' #h #_ #lt23 step_epair step_epair_steps -> begin
@@ -1107,7 +1015,7 @@ let rec destruct_steps_epair_e1
       lem_step_implies_steps (EPair e1 e2) (EPair e1' e2) h oev1;
       let lt1 : local_trace h = as_lt oev1 in
       let s2 : steps (EPair e1' e2) e' (h++lt1) lt23 = step_epair_steps in
-      lem_steps_preserve_is_value e1 e1' h lt1;
+      lem_step_preserve_indexed_safe e1 e1' h oev1;
       let (e1'', (| lt1', lt' |)) = destruct_steps_epair_e1 e1' e2 e' (h++lt1) lt23 s2 in
       lem_steps_transitive e1 e1' e1'' h lt1 lt1';
       lem_steps_transitive (EPair e1 e2) (EPair e1' e2) (EPair e1'' e2) h lt1 lt1';
@@ -1125,7 +1033,7 @@ let rec destruct_steps_epair_e2
   (st:steps (EPair e1' e2) e' h lt) :
   Pure (value * (lt2:local_trace h & local_trace (h++lt2)))
     (requires indexed_irred e' (h++lt) /\
-      (forall e2' lt2. steps e2 e2' h lt2 /\ indexed_irred e2' (h++lt2) ==> is_value e2'))
+      indexed_safe e2 h)
     (ensures fun (e2', (| lt2, lt' |)) ->
       steps e2 e2' h lt2 /\
       steps (EPair e1' e2) (EPair e1' e2') h lt2 /\
@@ -1136,6 +1044,7 @@ let rec destruct_steps_epair_e2
   match st with
   | SRefl (EPair e1' e2) h -> begin
     lem_irred_epair_implies_irred_e2 e1' e2 h;
+    assert (steps e2 e2 h []);
     (e2, (| [], lt |))
     end
   | STrans #e #f2 #e' #h #_ #lt23 step_epair step_epair_steps -> begin
@@ -1147,7 +1056,7 @@ let rec destruct_steps_epair_e2
       lem_step_implies_steps (EPair e1' e2) (EPair e1' e2') h oev2;
       let lt2 : local_trace h = as_lt oev2 in
       let s2 : steps (EPair e1' e2') e' (h++lt2) lt23 = step_epair_steps in
-      lem_steps_preserve_is_value e2 e2' h lt2;
+      lem_step_preserve_indexed_safe e2 e2' h oev2;
       let (e2'', (| lt2', lt' |)) = destruct_steps_epair_e2 e1' e2' e' (h++lt2) lt23 s2 in
       lem_steps_transitive e2 e2' e2'' h lt2 lt2';
       lem_steps_transitive (EPair e1' e2) (EPair e1' e2') (EPair e1' e2'') h lt2 lt2';
@@ -1172,9 +1081,8 @@ let lem_destruct_steps_epair
   Lemma (requires (steps (EPair e1' e2') e' h lt /\ indexed_irred e1' h /\ indexed_irred e2' h))
         (ensures ((EPair e1' e2') == e')) = admit ()
 
-let can_step_efst_when_safe (e12:closed_exp) (h:history) : Lemma
-  (requires
-    (forall e12' lt12. (steps e12 e12' h lt12 /\ indexed_irred e12' (h++lt12)) ==> (EPair? e12' /\ is_value e12')))
+let can_step_efst_when_reduced (e12:closed_exp) (h:history) (t1 t2:typ) : Lemma
+  (requires indexed_sem_expr_shape (TPair t1 t2) e12 h)
   (ensures (exists e' oev. step (EFst e12) e' h oev))
   =
   introduce indexed_irred e12 h ==> (exists e' oev. step (EFst e12) e' h oev) with _. begin
@@ -1196,10 +1104,11 @@ let rec destruct_steps_epair_fst
   (e':closed_exp)
   (h:history)
   (lt:local_trace h)
-  (st:steps (EFst e12) e' h lt) :
+  (st:steps (EFst e12) e' h lt) 
+  (t1 t2:typ) :
   Pure (value * (lt12:local_trace h & local_trace (h++lt12)))
     (requires indexed_irred e' (h++lt) /\
-      (forall e12' lt12. (steps e12 e12' h lt12 /\ indexed_irred e12' (h++lt12)) ==> (EPair? e12' /\ is_value e12'))) (** CA: not sure if necessary **)
+      indexed_sem_expr_shape (TPair t1 t2) e12 h) (** CA: not sure if necessary **)
     (ensures fun (e12', (| lt12, lt_f |)) ->
       indexed_irred e12' (h++lt12) /\
       steps e12 e12' h lt12 /\
@@ -1210,7 +1119,7 @@ let rec destruct_steps_epair_fst
     (decreases st)
   = match st with
     | SRefl (EFst e12) h -> begin
-      can_step_efst_when_safe e12 h;
+      can_step_efst_when_reduced e12 h t1 t2;
       false_elim ()
       end
     | STrans #e #f2 #e' #h #_ #lt23 step_efst step_efst_steps -> begin
@@ -1221,9 +1130,9 @@ let rec destruct_steps_epair_fst
         lem_step_implies_steps e12 e12' h oev12;
         lem_step_implies_steps (EFst e12) (EFst e12') h oev12;
         let lt12 : local_trace h = as_lt oev12 in
-        lem_steps_preserve_is_pair_value e12 e12' h lt12;
+        lem_step_preserve_indexed_sem_expr_shape e12 e12' h oev12 (TPair t1 t2);
         let s2 : steps (EFst e12') e' (h++lt12) lt23 = step_efst_steps in
-        let (e12'', (| lt12', lt_f |)) = destruct_steps_epair_fst e12' e' (h++lt12) lt23 s2 in
+        let (e12'', (| lt12', lt_f |)) = destruct_steps_epair_fst e12' e' (h++lt12) lt23 s2 t1 t2 in
         lem_steps_transitive e12 e12' e12'' h lt12 lt12';
         (e12'', (| (lt12 @ lt12'), lt_f |))
       end
@@ -1248,9 +1157,8 @@ let lem_destruct_steps_epair_fst
   Lemma (requires (steps (EFst (EPair e1 e2)) e' h lt /\ indexed_irred e1 h /\ indexed_irred e2 h))
         (ensures (e1 == e') /\ lt == []) = admit ()
 
-let can_step_esnd_when_safe (e12:closed_exp) (h:history) : Lemma
-  (requires
-    (forall e12' lt12. (steps e12 e12' h lt12 /\ indexed_irred e12' (h++lt12)) ==> (EPair? e12' /\ is_value e12')))
+let can_step_esnd_when_reduced (e12:closed_exp) (h:history) (t1 t2:typ) : Lemma
+  (requires indexed_sem_expr_shape (TPair t1 t2) e12 h)
   (ensures (exists e' oev. step (ESnd e12) e' h oev))
   =
   introduce indexed_irred e12 h ==> (exists e' oev. step (ESnd e12) e' h oev) with _. begin
@@ -1272,10 +1180,11 @@ let rec destruct_steps_epair_snd
   (e':closed_exp)
   (h:history)
   (lt:local_trace h)
-  (st:steps (ESnd e12) e' h lt) :
+  (st:steps (ESnd e12) e' h lt) 
+  (t1 t2:typ) :
   Pure (value * (lt12:local_trace h & local_trace (h++lt12)))
     (requires indexed_irred e' (h++lt) /\
-      (forall e12' lt12. (steps e12 e12' h lt12 /\ indexed_irred e12' (h++lt12)) ==> (EPair? e12' /\ is_value e12'))) (** CA: not sure if necessary **)
+      indexed_sem_expr_shape (TPair t1 t2) e12 h)
     (ensures fun (e12', (| lt12, lt_f |)) ->
       indexed_irred e12' (h++lt12) /\
       steps e12 e12' h lt12 /\
@@ -1286,7 +1195,7 @@ let rec destruct_steps_epair_snd
     (decreases st)
   = match st with
     | SRefl (ESnd e12) h -> begin
-      can_step_esnd_when_safe e12 h;
+      can_step_esnd_when_reduced e12 h t1 t2;
       false_elim ()
       end
     | STrans #e #f2 #e' #h #_ #lt23 step_esnd step_esnd_steps -> begin
@@ -1297,9 +1206,9 @@ let rec destruct_steps_epair_snd
         lem_step_implies_steps e12 e12' h oev12;
         lem_step_implies_steps (ESnd e12) (ESnd e12') h oev12;
         let lt12 : local_trace h = as_lt oev12 in
-        lem_steps_preserve_is_pair_value e12 e12' h lt12;
+        lem_step_preserve_indexed_sem_expr_shape e12 e12' h oev12 (TPair t1 t2);
         let s2 : steps (ESnd e12') e' (h++lt12) lt23 = step_esnd_steps in
-        let (e12'', (| lt12', lt_f |)) = destruct_steps_epair_snd e12' e' (h++lt12) lt23 s2 in
+        let (e12'', (| lt12', lt_f |)) = destruct_steps_epair_snd e12' e' (h++lt12) lt23 s2 t1 t2 in
         lem_steps_transitive e12 e12' e12'' h lt12 lt12';
         (e12'', (| (lt12 @ lt12'), lt_f |))
         end
@@ -1325,7 +1234,7 @@ let lem_destruct_steps_epair_snd
         (ensures (e2 == e') /\ lt == []) = admit ()
 
 let srefl_einl_implies_value (e12:closed_exp) (h:history) : Lemma
-  (requires (forall e12' lt12. steps e12 e12' h lt12 /\ indexed_irred e12' (h++lt12) ==> is_value e12') /\ indexed_irred (EInl e12) h)
+  (requires indexed_safe e12 h /\ indexed_irred (EInl e12) h)
   (ensures is_value (EInl e12))
   =
   introduce indexed_irred e12 h ==> is_value (EInl e12) with _. begin
@@ -1349,15 +1258,15 @@ let rec destruct_steps_einl
   (st:steps (EInl e12) e' h lt) :
   Pure (value * (lt12:local_trace h & local_trace (h++lt12)))
     (requires indexed_irred e' (h++lt) /\
-      (forall e12' lt12. steps e12 e12' h lt12 /\ indexed_irred e12' (h++lt12) ==> is_value e12'))
+      indexed_safe e12 h)
     (ensures fun (e12', (| lt12, lt_f |)) ->
-              indexed_irred e12' (h++lt12) /\
-              steps e12 e12' h lt12 /\
-              steps (EInl e12) (EInl e12') h lt12 /\
-              is_closed (EInl e12') /\
-              steps (EInl e12') e' (h++lt12) lt_f /\
-              lt == (lt12 @ lt_f) /\
-              (indexed_irred e12 h ==> (lt12 == [] /\ e12 == e12')))
+      indexed_irred e12' (h++lt12) /\
+      steps e12 e12' h lt12 /\
+      steps (EInl e12) (EInl e12') h lt12 /\
+      is_closed (EInl e12') /\
+      steps (EInl e12') e' (h++lt12) lt_f /\
+      lt == (lt12 @ lt_f) /\
+      (indexed_irred e12 h ==> (lt12 == [] /\ e12 == e12')))
     (decreases st)
   = match st with
     | SRefl (EInl e12) h -> begin
@@ -1372,7 +1281,7 @@ let rec destruct_steps_einl
       lem_step_implies_steps e12 e12' h oev12;
       lem_step_implies_steps (EInl e12) (EInl e12') h oev12;
       let lt12 : local_trace h = as_lt oev12 in
-      lem_steps_preserve_is_value e12 e12' h lt12;
+      lem_step_preserve_indexed_safe e12 e12' h oev12;
       let s2 : steps (EInl e12') e' (h++lt12) lt23 = step_einl_steps in
       let (e12'', (| lt12', lt_f |)) = destruct_steps_einl e12' e' (h++lt12) lt23 s2 in
       lem_steps_transitive e12 e12' e12'' h lt12 lt12';
@@ -1398,7 +1307,7 @@ let lem_destruct_steps_einl
   end
 
 let srefl_einr_implies_value (e12:closed_exp) (h:history) : Lemma
-  (requires (forall e12' lt12. steps e12 e12' h lt12 /\ indexed_irred e12' (h++lt12) ==> is_value e12') /\ indexed_irred (EInr e12) h)
+  (requires indexed_safe e12 h /\ indexed_irred (EInr e12) h)
   (ensures is_value (EInr e12))
   =
   introduce indexed_irred e12 h ==> is_value (EInr e12) with _. begin
@@ -1422,15 +1331,15 @@ let rec destruct_steps_einr
   (st:steps (EInr e12) e' h lt) :
   Pure (value * (lt12:local_trace h & local_trace (h++lt12)))
     (requires indexed_irred e' (h++lt) /\
-              (forall e12' lt12. steps e12 e12' h lt12 /\ indexed_irred e12' (h++lt12) ==> is_value e12'))
+      indexed_safe e12 h)
     (ensures fun (e12', (| lt12, lt_f |)) ->
-              indexed_irred e12' (h++lt12) /\
-              steps e12 e12' h lt12 /\
-              steps (EInr e12) (EInr e12') h lt12 /\
-              is_closed (EInr e12') /\
-              steps (EInr e12') e' (h++lt12) lt_f /\
-              lt == (lt12 @ lt_f) /\
-              (indexed_irred e12 h ==> (lt12 == [] /\ e12 == e12')))
+      indexed_irred e12' (h++lt12) /\
+      steps e12 e12' h lt12 /\
+      steps (EInr e12) (EInr e12') h lt12 /\
+      is_closed (EInr e12') /\
+      steps (EInr e12') e' (h++lt12) lt_f /\
+      lt == (lt12 @ lt_f) /\
+      (indexed_irred e12 h ==> (lt12 == [] /\ e12 == e12')))
     (decreases st)
   = match st with
     | SRefl (EInr e12) h -> begin
@@ -1445,7 +1354,7 @@ let rec destruct_steps_einr
       lem_step_implies_steps e12 e12' h oev12;
       lem_step_implies_steps (EInr e12) (EInr e12') h oev12;
       let lt12 : local_trace h = as_lt oev12 in
-      lem_steps_preserve_is_value e12 e12' h lt12;
+      lem_step_preserve_indexed_safe e12 e12' h oev12;
       let s2 : steps (EInr e12') e' (h++lt12) lt23 = step_einr_steps in
       let (e12'', (| lt12', lt_f |)) = destruct_steps_einr e12' e' (h++lt12) lt23 s2 in
       lem_steps_transitive e12 e12' e12'' h lt12 lt12';
@@ -1470,9 +1379,8 @@ let lem_destruct_steps_einr
     )
   end
 
-let can_step_ecase_when_safe (e_case:closed_exp) (e_lc:exp{is_closed (ELam e_lc)}) (e_rc:exp{is_closed (ELam e_rc)}) (h:history) : Lemma
-  (requires
-    (forall e_case' lt'. steps e_case e_case' h lt' /\ indexed_irred e_case' (h++lt') ==> ((EInl? e_case' \/ EInr? e_case') /\ is_value e_case')))
+let can_step_ecase_when_safe (e_case:closed_exp) (e_lc:exp{is_closed (ELam e_lc)}) (e_rc:exp{is_closed (ELam e_rc)}) (h:history) (t1 t2:typ) : Lemma
+  (requires indexed_sem_expr_shape (TSum t1 t2) e_case h)
   (ensures (exists e' oev. step (ECase e_case e_lc e_rc) e' h oev))
   =
   introduce indexed_irred e_case h ==> (exists e' oev. step (ECase e_case e_lc e_rc) e' h oev) with _. begin
@@ -1508,10 +1416,11 @@ let rec destruct_steps_ecase
   (e':closed_exp)
   (h:history)
   (lt:local_trace h)
-  (st:steps (ECase e_case e_lc e_rc) e' h lt) :
+  (st:steps (ECase e_case e_lc e_rc) e' h lt) 
+  (t1 t2:typ) :
   Pure (closed_exp * (lt1:local_trace h & (local_trace (h++lt1) * local_trace (h++lt1))))
     (requires indexed_irred e' (h++lt) /\
-      (forall e_case' lt'. steps e_case e_case' h lt' /\ indexed_irred e_case' (h++lt') ==> ((EInl? e_case' \/ EInr? e_case') /\ is_value e_case')))
+      indexed_sem_expr_shape (TSum t1 t2) e_case h)
     (ensures fun (e_case', (| lt1, (lt2, lt3) |)) ->
       indexed_irred e_case' (h++lt1) /\
       steps e_case e_case' h lt1 /\
@@ -1531,7 +1440,7 @@ let rec destruct_steps_ecase
     (decreases st)
   = match st with
     | SRefl (ECase e_case e_lc e_rc) h -> begin
-      can_step_ecase_when_safe e_case e_lc e_rc h;
+      can_step_ecase_when_safe e_case e_lc e_rc h t1 t2;
       false_elim ()
       end
     | STrans #e #f2 #e' #h #_ #lt23 step_ecase step_ecase_steps -> begin
@@ -1542,9 +1451,9 @@ let rec destruct_steps_ecase
         lem_step_implies_steps e_case e_case' h oev1;
         lem_step_implies_steps (ECase e_case e_lc e_rc) (ECase e_case' e_lc e_rc) h oev1;
         let lt1 : local_trace h = as_lt oev1 in
-        lem_steps_preserve_is_sum_value e_case e_case' h lt1;
+        lem_step_preserve_indexed_sem_expr_shape e_case e_case' h oev1 (TSum t1 t2);
         let s2 : steps (ECase e_case' e_lc e_rc) e' (h++lt1) lt23 = step_ecase_steps in
-        let (e_case'', (| lt1', (lt2, lt3) |)) = destruct_steps_ecase e_case' e_lc e_rc e' (h++lt1) lt23 s2 in
+        let (e_case'', (| lt1', (lt2, lt3) |)) = destruct_steps_ecase e_case' e_lc e_rc e' (h++lt1) lt23 s2 t1 t2 in
         lem_steps_transitive e_case e_case' e_case'' h lt1 lt1';
         lem_steps_transitive (ECase e_case e_lc e_rc) (ECase e_case' e_lc e_rc) (ECase e_case'' e_lc e_rc) h lt1 lt1';
         match e_case'' with
@@ -1581,7 +1490,7 @@ let can_step_eread_fd (fd:closed_exp{EFileDescr? fd}) (h:history) :
 
 let can_step_eread (fd:closed_exp) (h:history) :
   Lemma
-  (requires (forall fd' lt'. steps fd fd' h lt' /\ indexed_irred fd' (h++lt') ==> (EFileDescr? fd' /\ is_value fd')))  
+  (requires indexed_sem_expr_shape TFileDescr fd h)  
   (ensures (exists e' oev. step (ERead fd) e' h oev))
   =
   introduce indexed_irred fd h ==> (exists e' oev. step (ERead fd) e' h oev) with _. begin
@@ -1607,7 +1516,7 @@ let rec destruct_steps_eread_fd
   (st:steps (ERead fd) e' h lt) :
   Pure (value * (lt1:local_trace h & local_trace (h++lt1)))
   (requires indexed_irred e' (h++lt) /\
-    (forall fd' lt'. (steps fd fd' h lt' /\ indexed_irred fd' (h++lt')) ==> (EFileDescr? fd' /\ is_value fd')))
+    indexed_sem_expr_shape TFileDescr fd h)
   (ensures fun (fd', (| lt1, lt' |)) ->
     EFileDescr? fd' /\
     steps fd fd' h lt1 /\
@@ -1629,7 +1538,7 @@ let rec destruct_steps_eread_fd
       lem_step_implies_steps (ERead fd) (ERead fd') h oev;
       let lt1 : local_trace h = as_lt oev in
       let s2 : steps (ERead fd') e' (h++lt1) lt23 = step_eread_steps in
-      lem_steps_preserve_is_file_descr_value fd fd' h lt1;
+      lem_step_preserve_indexed_sem_expr_shape fd fd' h oev TFileDescr;
       let (fd'', (| lt1', lt' |)) = destruct_steps_eread_fd fd' e' (h++lt1) lt23 s2 in
       lem_steps_transitive fd fd' fd'' h lt1 lt1';
       lem_steps_transitive (ERead fd) (ERead fd') (ERead fd'') h lt1 lt1';
@@ -1669,7 +1578,7 @@ let destruct_steps_eread
         lem_step_implies_steps (ERead (get_efd fd)) (EInl ETrue) h (Some (EvRead fd (Inl true)));
         let lt' : local_trace h = [EvRead fd (Inl true)] in
         let s2 : steps (EInl ETrue) e' (h++lt') lt23 = step_eread_steps in
-        lem_value_preserves_value ETrue (h++lt');
+        lem_value_preserves_value ETrue (h++lt') TBool;
         let (e12', (| lt12, lt_f |)) = destruct_steps_einl ETrue e' (h++lt') lt23 s2 in
         (f2, (| lt', (lt12 @ lt_f, [], []) |))
         end
@@ -1678,7 +1587,7 @@ let destruct_steps_eread
         lem_step_implies_steps (ERead (get_efd fd)) (EInl EFalse) h (Some (EvRead fd (Inl false)));
         let lt' : local_trace h = [EvRead fd (Inl false)] in
         let s2 : steps (EInl EFalse) e' (h++lt') lt23 = step_eread_steps in
-        lem_value_preserves_value EFalse (h++lt');
+        lem_value_preserves_value EFalse (h++lt') TBool;
         let (e12', (| lt12, lt_f |)) = destruct_steps_einl EFalse e' (h++lt') lt23 s2 in
         (f2, (| lt', ([], lt12 @ lt_f, []) |))
         end
@@ -1687,7 +1596,7 @@ let destruct_steps_eread
         lem_step_implies_steps (ERead (get_efd fd)) (EInr EUnit) h (Some (EvRead fd (Inr ())));
         let lt' : local_trace h = [EvRead fd (Inr ())] in
         let s2 : steps (EInr EUnit) e' (h++lt') lt23 = step_eread_steps in
-        lem_value_preserves_value EUnit (h++lt');
+        lem_value_preserves_value EUnit (h++lt') TUnit;
         let (e12', (| lt12, lt_f |)) = destruct_steps_einr EUnit e' (h++lt') lt23 s2 in
         (f2, (| lt', ([], [], lt12 @ lt_f) |))
         end
@@ -1740,7 +1649,7 @@ let rec destruct_steps_ewrite_fd
   (st:steps (EWrite fd arg) e' h lt) :
   Pure (value * (lt1:local_trace h & local_trace (h++lt1)))
     (requires indexed_irred e' (h++lt) /\
-      (forall fd' lt'. (steps fd fd' h lt' /\ indexed_irred fd' (h++lt')) ==> (EFileDescr? fd' /\ is_value fd')))
+      indexed_sem_expr_shape TFileDescr fd h)
     (ensures fun (fd', (| lt1, lt' |)) ->
       EFileDescr? fd' /\
       steps fd fd' h lt1 /\
@@ -1762,7 +1671,7 @@ let rec destruct_steps_ewrite_fd
       lem_step_implies_steps (EWrite fd arg) (EWrite fd' arg) h oev;
       let lt1 : local_trace h = as_lt oev in
       let s2 : steps (EWrite fd' arg) e' (h++lt1) lt23 = step_ewrite_steps in
-      lem_steps_preserve_is_file_descr_value fd fd' h lt1;
+      lem_step_preserve_indexed_sem_expr_shape fd fd' h oev TFileDescr;
       let (fd'', (| lt1', lt' |)) = destruct_steps_ewrite_fd fd' arg e' (h++lt1) lt23 s2 in
       lem_steps_transitive fd fd' fd'' h lt1 lt1';
       lem_steps_transitive (EWrite fd arg) (EWrite fd' arg) (EWrite fd'' arg) h lt1 lt1';
@@ -1780,7 +1689,7 @@ let rec destruct_steps_ewrite_arg
   (st:steps (EWrite fd' arg) e' h lt) :
   Pure (value * (lt1:local_trace h & local_trace (h++lt1)))
     (requires indexed_irred e' (h++lt) /\
-      (forall arg' lt'. steps arg arg' h lt' /\ indexed_irred arg' (h++lt') ==> (ETrue? arg' \/ EFalse? arg')))
+      indexed_sem_expr_shape TBool arg h)
     (ensures fun (arg', (| lt1, lt' |)) ->
       (ETrue? arg' \/ EFalse? arg') /\
       steps arg arg' h lt1 /\
@@ -1802,7 +1711,7 @@ let rec destruct_steps_ewrite_arg
       lem_step_implies_steps (EWrite fd' arg) (EWrite fd' arg') h oev;
       let lt1 : local_trace h = as_lt oev in
       let s2 : steps (EWrite fd' arg') e' (h++lt1) lt23 = step_ewrite_steps in
-      lem_steps_preserve_is_bool_value arg arg' h lt1;
+      lem_step_preserve_indexed_sem_expr_shape arg arg' h oev TBool;
       let (arg'', (| lt1', lt' |)) = destruct_steps_ewrite_arg fd' arg' e' (h++lt1) lt23 s2 in
       lem_steps_transitive arg arg' arg'' h lt1 lt1';
       lem_steps_transitive (EWrite fd' arg) (EWrite fd' arg') (EWrite fd' arg'') h lt1 lt1';
@@ -1847,7 +1756,7 @@ let destruct_steps_ewrite
         lem_value_is_irred arg';
         let lt' : local_trace h = [EvWrite (fd_t, get_bool arg') (Inl ())] in
         let s2 : steps (EInl EUnit) e' (h++lt') lt23 = step_ewrite_steps in
-        lem_value_preserves_value EUnit (h++lt');
+        lem_value_preserves_value EUnit (h++lt') TUnit;
         let (e12', (| lt12, lt_f |)) = destruct_steps_einl EUnit e' (h++lt') lt23 s2 in
         (f2, (| lt', (lt12 @ lt_f, []) |))
         end
@@ -1857,7 +1766,7 @@ let destruct_steps_ewrite
         lem_value_is_irred arg';
         let lt' : local_trace h = [EvWrite (fd_t, get_bool arg') (Inr ())] in
         let s2 : steps (EInr EUnit) e' (h++lt') lt23 = step_ewrite_steps in
-        lem_value_preserves_value EUnit (h++lt');
+        lem_value_preserves_value EUnit (h++lt') TUnit;
         let (e12', (| lt12, lt_f |)) = destruct_steps_einr EUnit e' (h++lt') lt23 s2 in
         (f2, (| lt', ([], lt12 @ lt_f) |))
         end
@@ -1875,7 +1784,7 @@ let can_step_eopen_str (str:closed_exp{ETrue? str \/ EFalse? str}) (h:history) :
 
 let can_step_eopen (str:closed_exp) (h:history) :
   Lemma
-  (requires (forall str' lt'. steps str str' h lt' /\ indexed_irred str' (h++lt') ==> (ETrue? str' \/ EFalse? str')))  
+  (requires indexed_sem_expr_shape TBool str h)  
   (ensures (exists e' oev. step (EOpen str) e' h oev))
   =
   introduce indexed_irred str h ==> (exists e' oev. step (EOpen str) e' h oev) with _. begin
@@ -1900,7 +1809,7 @@ let rec destruct_steps_eopen_str
   (st:steps (EOpen str) e' h lt) :
   Pure (value * (lt1:local_trace h & local_trace (h++lt1)))
   (requires indexed_irred e' (h++lt) /\
-    (forall str' lt'. (steps str str' h lt' /\ indexed_irred str' (h++lt')) ==> (ETrue? str' \/ EFalse? str')))
+    indexed_sem_expr_shape TBool str h)
   (ensures fun (str', (| lt1, lt' |)) ->
     (ETrue? str' \/ EFalse? str') /\
     steps str str' h lt1 /\
@@ -1922,7 +1831,7 @@ let rec destruct_steps_eopen_str
       lem_step_implies_steps (EOpen str) (EOpen str') h oev;
       let lt1 : local_trace h = as_lt oev in
       let s2 : steps (EOpen str') e' (h++lt1) lt23 = step_eopen_steps in
-      lem_steps_preserve_is_bool_value str str' h lt1;
+      lem_step_preserve_indexed_sem_expr_shape str str' h oev TBool;
       let (str'', (| lt1', lt' |)) = destruct_steps_eopen_str str' e' (h++lt1) lt23 s2 in
       lem_steps_transitive str str' str'' h lt1 lt1';
       lem_steps_transitive (EOpen str) (EOpen str') (EOpen str'') h lt1 lt1';
@@ -1962,7 +1871,7 @@ let destruct_steps_eopen
         lem_step_implies_steps (EOpen str') (EInl (get_efd (fresh_fd h))) h (Some (EvOpen (get_bool str') (Inl (fresh_fd h))));
         let lt' : local_trace h = [EvOpen (get_bool str') (Inl (fresh_fd h))] in
         let s2 : steps (EInl (get_efd (fresh_fd h))) e' (h++lt') lt23 = step_eopen_steps in
-        lem_value_preserves_value (get_efd (fresh_fd h)) (h++lt');
+        lem_value_preserves_value (get_efd (fresh_fd h)) (h++lt') TFileDescr;
         let (e12', (| lt12, lt_f |)) = destruct_steps_einl (get_efd (fresh_fd h)) e' (h++lt') lt23 s2 in
         (f2, (| lt', (lt12 @ lt_f, []) |))
         end
@@ -1971,7 +1880,7 @@ let destruct_steps_eopen
         lem_step_implies_steps (EOpen str') (EInr EUnit) h (Some (EvOpen (get_bool str') (Inr ())));
         let lt' : local_trace h = [EvOpen (get_bool str') (Inr ())] in
         let s2 : steps (EInr EUnit) e' (h++lt') lt23 = step_eopen_steps in
-        lem_value_preserves_value EUnit (h++lt');
+        lem_value_preserves_value EUnit (h++lt') TUnit;
         let (e12', (| lt12, lt_f |)) = destruct_steps_einr EUnit e' (h++lt') lt23 s2 in
         (f2, (| lt', ([], lt12 @ lt_f) |))
         end
@@ -1980,7 +1889,7 @@ let destruct_steps_eopen
 
 let can_step_eclose (fd:closed_exp) (h:history) :
   Lemma
-  (requires (forall fd' lt'. steps fd fd' h lt' /\ indexed_irred fd' (h++lt') ==> (EFileDescr? fd' /\ is_value fd')))  
+  (requires indexed_sem_expr_shape TFileDescr fd h)  
   (ensures (exists e' oev. step (EClose fd) e' h oev))
   =
   introduce indexed_irred fd h ==> (exists e' oev. step (EClose fd) e' h oev) with _. begin
@@ -2005,7 +1914,7 @@ let rec destruct_steps_eclose_fd
   (st:steps (EClose fd) e' h lt) :
   Pure (value * (lt1:local_trace h & local_trace (h++lt1)))
   (requires indexed_irred e' (h++lt) /\
-    (forall fd' lt'. (steps fd fd' h lt' /\ indexed_irred fd' (h++lt')) ==> (EFileDescr? fd' /\ is_value fd')))
+    indexed_sem_expr_shape TFileDescr fd h)
   (ensures fun (fd', (| lt1, lt' |)) ->
     EFileDescr? fd' /\
     steps fd fd' h lt1 /\
@@ -2027,7 +1936,7 @@ let rec destruct_steps_eclose_fd
       lem_step_implies_steps (EClose fd) (EClose fd') h oev;
       let lt1 : local_trace h = as_lt oev in
       let s2 : steps (EClose fd') e' (h++lt1) lt23 = step_eclose_steps in
-      lem_steps_preserve_is_file_descr_value fd fd' h lt1;
+      lem_step_preserve_indexed_sem_expr_shape fd fd' h oev TFileDescr;
       let (fd'', (| lt1', lt' |)) = destruct_steps_eclose_fd fd' e' (h++lt1) lt23 s2 in
       lem_steps_transitive fd fd' fd'' h lt1 lt1';
       lem_steps_transitive (EClose fd) (EClose fd') (EClose fd'') h lt1 lt1';
@@ -2074,7 +1983,7 @@ let destruct_steps_eclose
         lem_step_implies_steps (EClose (get_efd fd)) (EInl EUnit) h (Some (EvClose fd (Inl ())));
         let lt' : local_trace h = [EvClose fd (Inl ())] in
         let s2 : steps (EInl EUnit) e' (h++lt') lt23 = step_eclose_steps in
-        lem_value_preserves_value EUnit (h++lt');
+        lem_value_preserves_value EUnit (h++lt') TUnit;
         let (e12', (| lt12, lt_f |)) = destruct_steps_einl EUnit e' (h++lt') lt23 s2 in
         (f2, (| lt', (lt12 @ lt_f, []) |))
         end
@@ -2083,378 +1992,9 @@ let destruct_steps_eclose
         lem_step_implies_steps (EClose (get_efd fd)) (EInr EUnit) h (Some (EvClose fd (Inr ())));
         let lt' : local_trace h = [EvClose fd (Inr ())] in
         let s2 : steps (EInr EUnit) e' (h++lt') lt23 = step_eclose_steps in
-        lem_value_preserves_value EUnit (h++lt');
+        lem_value_preserves_value EUnit (h++lt') TUnit;
         let (e12', (| lt12, lt_f |)) = destruct_steps_einr EUnit e' (h++lt') lt23 s2 in
         (f2, (| lt', ([], lt12 @ lt_f) |))
         end
       end
 #pop-options
-
-// HISTORY INDEPENDENCE PROOFS:
-(*
-let rec construct_step (#e #e':closed_exp) (#h:history) (#oev:option (event_h h)) (st:step e e' h oev) (h':history) (oev':option (event_h h')) : Pure (step e e' h' oev')
-  (requires step e e' h oev /\
-            (None? oev ==> None? oev') /\
-            ((Some? oev /\ (EvRead? (Some?.v oev) \/ EvWrite? (Some?.v oev))) ==> (oev == oev')) /\
-            ((Some? oev /\ ~(EvRead? (Some?.v oev) \/ EvWrite? (Some?.v oev))) ==> (test_event h' (Some?.v oev) ==> (oev == oev'))) /\
-            ((Some? oev /\ ~(EvRead? (Some?.v oev) \/ EvWrite? (Some?.v oev))) ==> (~(test_event h' (Some?.v oev)) ==> (None? oev'))))
-            // TODO: this is not correct - look at corresponding_event for correct spec
-  (ensures fun _ -> step e e' h' oev')
-  (decreases st) =
-  match st with
-  | AppRight e1 hst -> begin
-    let hst' = construct_step hst h' oev' in
-    AppRight e1 hst'
-    end
-  | AppLeft e2 hst -> begin
-    let hst' = construct_step hst h' oev' in
-    AppLeft e2 hst'
-    end
-  | Beta e11 e2 h -> Beta e11 e2 h'
-  | IfCond e2 e3 hst -> begin
-    let hst' = construct_step hst h' oev' in
-    IfCond e2 e3 hst'
-    end
-  | IfTrue e2 e3 h -> IfTrue e2 e3 h'
-  | IfFalse e2 e3 h -> IfFalse e2 e3 h'
-  | PairLeft e2 hst -> begin
-    let hst' = construct_step hst h' oev' in
-    PairLeft e2 hst'
-    end
-  | PairRight e1 hst -> begin
-    let hst' = construct_step hst h' oev' in
-    PairRight e1 hst'
-    end
-  | FstPair hst -> begin
-    let hst' = construct_step hst h' oev' in
-    FstPair hst'
-    end
-  | FstPairReturn #e1 #e2 h -> FstPairReturn #e1 #e2 h'
-  | SndPair hst -> begin
-    let hst' = construct_step hst h' oev' in
-    SndPair hst'
-    end
-  | SndPairReturn #e1 #e2 h -> SndPairReturn #e1 #e2 h'
-  | SCase e2 e3 hst -> begin
-    let hst' = construct_step hst h' oev' in
-    SCase e2 e3 hst'
-    end
-  | SInl hst -> begin
-    let hst' = construct_step hst h' oev' in
-    SInl hst'
-    end
-  | SInlReturn e1 e2 e3 h -> SInlReturn e1 e2 e3 h'
-  | SInr hst -> begin
-    let hst' = construct_step hst h' oev' in
-    SInr hst'
-    end
-  | SInrReturn e1 e2 e3 h -> SInrReturn e1 e2 e3 h'
-  | SRead b h -> SRead b h'
-  | SWrite hst -> begin
-    let hst' = construct_step hst h' oev' in
-    SWrite hst'
-    end
-  | SWriteReturn arg r h -> SWriteReturn arg r h'
-  | SOpen hst -> begin
-    let hst' = construct_step hst h' oev' in
-    SOpen hst'
-    end
-  | SOpenReturnSuccess str h -> SOpenReturnSuccess str h'
-  | SOpenReturnFail str h -> SOpenReturnFail str h'
-  | SClose hst -> begin
-    let hst' = construct_step hst h' oev' in
-    SClose hst'
-    end
-  | SCloseReturn file_descr r h -> SCloseReturn file_descr r h'
-
-let rec construct_option_ev (#e #e':closed_exp) (#h:history) (#oev:option (event_h h)) (st:step e e' h oev) (h':history) : Pure (option (event_h h'))
-  (requires step e e' h oev)
-  (ensures fun (oev') ->
-    (step e e' h' oev') /\
-    (None? oev ==> None? oev') /\
-    ((Some? oev /\ (EvRead? (Some?.v oev) \/ EvWrite? (Some?.v oev))) ==> (oev == oev')) /\
-    ((Some? oev /\ ~(EvRead? (Some?.v oev) \/ EvWrite? (Some?.v oev))) ==> (test_event h' (Some?.v oev) ==> (oev == oev'))) /\
-    ((Some? oev /\ ~(EvRead? (Some?.v oev) \/ EvWrite? (Some?.v oev))) ==> (~(test_event h' (Some?.v oev)) ==> (None? oev'))))
-  (decreases st) =
-  match st with
-  | AppRight e1 #e2 #e2' #h #oev2 hst2 -> begin
-    let oev2' = construct_option_ev hst2 h' in
-    let hst' : step e2 e2' h' oev2' = construct_step hst2 h' oev2' in
-    let _ : step e e' h' oev2' = AppRight e1 hst' in
-    oev2'
-    end
-  | AppLeft #e1 e2 #e1' #h #oev1 hst1 -> begin
-    let oev1' = construct_option_ev hst1 h' in
-    let hst' : step e1 e1' h' oev1' = construct_step hst1 h' oev1' in
-    let _ : step e e' h' oev1' = AppLeft e2 hst' in
-    oev1'
-    end
-  | Beta e11 e2 h -> begin
-    let _ : step e e' h' None = Beta e11 e2 h' in
-    None
-    end
-  | IfCond #e1 e2 e3 #e1' #h #oev1 hst1 -> begin
-    let oev1' = construct_option_ev hst1 h' in
-    let hst' : step e1 e1' h' oev1' = construct_step hst1 h' oev1' in
-    let _ : step e e' h' oev1' = IfCond e2 e3 hst' in
-    oev1'
-    end
-  | IfTrue e2 e3 h -> begin
-    let _ : step e e' h' None = IfTrue e2 e3 h' in
-    None
-    end
-  | IfFalse e2 e3 h -> begin
-    let _ : step e e' h' None = IfFalse e2 e3 h' in
-    None
-    end
-  | PairLeft #e1 e2 #e1' #h #oev1 hst1 -> begin
-    let oev1' = construct_option_ev hst1 h' in
-    let hst' : step e1 e1' h' oev1' = construct_step hst1 h' oev1' in
-    let _ : step e e' h' oev1' = PairLeft e2 hst' in
-    oev1'
-    end
-  | PairRight e1 #e2 #e2' #h #oev2 hst2 -> begin
-    let oev2' = construct_option_ev hst2 h' in
-    let hst' : step e2 e2' h' oev2' = construct_step hst2 h' oev2' in
-    let _ : step e e' h' oev2' = PairRight e1 hst' in
-    oev2'
-    end
-  | FstPair #e1 #e1' #h #oev hst -> begin
-    let oev' = construct_option_ev hst h' in
-    let hst' : step e1 e1' h' oev' = construct_step hst h' oev' in
-    let _ : step e e' h' oev' = FstPair hst' in
-    oev'
-    end
-  | FstPairReturn #e1 #e2 h -> begin
-    let _ : step e e' h' None = FstPairReturn #e1 #e2 h' in
-    None
-    end
-  | SndPair #e2 #e2' #h #oev hst -> begin
-    let oev' = construct_option_ev hst h' in
-    let hst' : step e2 e2' h' oev' = construct_step hst h' oev' in
-    let _ : step e e' h' oev' = SndPair hst' in
-    oev'
-    end
-  | SndPairReturn #e1 #e2 h -> begin
-    let _ : step e e' h' None = SndPairReturn #e1 #e2 h' in
-    None
-    end
-  | SCase #e1 e2 e3 #e1' #h #oev1 hst1 -> begin
-    let oev1' = construct_option_ev hst1 h' in
-    let hst' : step e1 e1' h' oev1' = construct_step hst1 h' oev1' in
-    let _ : step e e' h' oev1' = SCase e2 e3 hst' in
-    oev1'
-    end
-  | SInl #e12 #e12' #h #oev hst -> begin
-    let oev' = construct_option_ev hst h' in
-    let hst' : step e12 e12' h' oev' = construct_step hst h' oev' in
-    let _ : step e e' h' oev' = SInl hst' in
-    oev'
-    end
-  | SInlReturn e1 e2 e3 h -> begin
-    let _ : step e e' h' None = SInlReturn e1 e2 e3 h' in
-    None
-    end
-  | SInr #e12 #e12' #h #oev hst -> begin
-    let oev' = construct_option_ev hst h' in
-    let hst' : step e12 e12' h' oev' = construct_step hst h' oev' in
-    let _ : step e e' h' oev' = SInr hst' in
-    oev'
-    end
-  | SInrReturn e1 e2 e3 h -> begin
-    let _ : step e e' h' None = SInrReturn e1 e2 e3 h' in
-    None
-    end
-  | SRead b h -> begin
-    let _ : step e e' h' (Some (EvRead () b)) = SRead b h' in
-    Some (EvRead () b)
-    end
-  | SWrite #arg #arg' #h #oev hst -> begin
-    let oev' = construct_option_ev hst h' in
-    let hst' : step arg arg' h' oev' = construct_step hst h' oev' in
-    let _ : step e e' h' oev' = SWrite hst' in
-    oev'
-    end
-  | SWriteReturn arg r h -> begin
-    let _ : step e e' h' (Some (EvWrite (get_bool arg) r)) = SWriteReturn arg r h' in
-    Some (EvWrite (get_bool arg) r)
-    end
-  | SOpen #str #str' #h #oev hst -> begin
-    let oev' = construct_option_ev hst h' in
-    let hst' : step str str' h' oev' = construct_step hst h' oev' in
-    let _ : step e e' h' oev' = SOpen hst' in
-    oev'
-    end
-  | SOpenReturnSuccess str h -> begin
-    let _ : step e e' h' (Some (EvOpen (get_bool str) (Inl (fresh_fd h)))) = SOpenReturnSuccess str h' in
-    (Some (EvOpen (get_bool str) (Inl (fresh_fd h))))
-    end
-  | SOpenReturnFail str h -> begin
-    let _ : step e e' h' (Some (EvOpen (get_bool str) (Inr ()))) = SOpenReturnFail str h' in
-    (Some (EvOpen (get_bool str) (Inr ())))
-    end
-  | SClose #fd #fd' #h #oev hst -> begin
-    let oev' = construct_option_ev hst h' in
-    let hst' : step fd fd' h' oev' = construct_step hst h' oev' in
-    let _ : step e e' h' oev' = SClose hst' in
-    oev'
-    end
-  | SCloseReturn file_descr r h -> begin
-    let _ : step e e' h' (Some (EvClose file_descr r)) = SCloseReturn file_descr r h' in
-    Some (EvClose file_descr r)
-    end
-
-let step_history_independence (#e #e':closed_exp) (#h:history) (#oev:option (event_h h)) (st:step e e' h oev) :
-  Lemma (ensures forall h'. exists oev'. step e e' h' oev' /\ (None? oev <==> None? oev')) =
-  introduce forall h'. exists oev'. step e e' h' oev' /\ (None? oev <==> None? oev') with begin
-    assert (step e e' h' (construct_option_ev st h'))
-  end
-
-let rec construct_local_trace (#e #e':closed_exp) (#h:history) (#lt:local_trace h) (st:steps e e' h lt) (h':history) : Pure (local_trace h')
-  (requires steps e e' h lt)
-  (ensures fun lt' ->
-    steps e e' h' lt' /\
-    (lt == [] <==> lt' == []))
-  (decreases st) =
-  match st with
-  | SRefl _ _ -> []
-  | STrans #e #e_i #e' #h #oev #_ e_step steps_to_e' -> begin
-    step_history_independence e_step;
-    let oev' = construct_option_ev e_step h' in
-    assert (oev == oev');
-    lem_step_implies_steps e e_i h' oev';
-    let lt_ = as_lt oev' in
-    let rest_of_trace = construct_local_trace steps_to_e' (h'++lt_) in
-    lem_steps_transitive e e_i e' h' lt_ rest_of_trace;
-    match oev' with
-    | Some ev' -> [ev'] @ rest_of_trace
-    | None -> rest_of_trace
-    end
-
-let steps_history_independence (#e #e':closed_exp) (#h:history) (#lt:local_trace h) (sts:steps e e' h lt) :
-  Lemma (ensures forall h'. exists lt'. steps e e' h' lt' /\ (lt == [] <==> lt' == [])) =
-  introduce forall h'. exists lt'. steps e e' h' lt' /\ (lt == [] <==> lt' == []) with begin
-    assert (steps e e' h' (construct_local_trace sts h'))
- end
-
-let indexed_can_step_history_independence (e:closed_exp) (h:history) :
-  Lemma (requires indexed_can_step e h)
-        (ensures forall h'. indexed_can_step e h') =
-  introduce forall h'. exists (e':closed_exp) (oev:option (event_h h')). step e e' h' oev with begin
-    eliminate exists e' oev. step e e' h oev
-    returns exists e' oev. step e e' h' oev with _. begin
-      bind_squash #(step e e' h oev) () (fun st ->
-        assert (step e e' h' (construct_option_ev st h'))
-      )
-    end
-  end
-
-let lem_step_preserve_safe (e e':closed_exp) (h:history) (oev:option (event_h h)) :
-  Lemma (requires safe e /\ step e e' h oev)
-        (ensures safe e') =
-  introduce forall e'' h' lt'. steps e' e'' h' lt' ==> (is_value e'' \/ indexed_can_step e'' (h'++lt')) with begin
-    introduce steps e' e'' h' lt' ==> (is_value e'' \/ indexed_can_step e'' (h'++lt')) with _. begin
-      bind_squash #(steps e' e'' h' lt') () (fun sts ->
-      steps_history_independence sts;
-      assert (forall h_. exists lt_. steps e' e'' h_ lt_);
-      let lt_ev = as_lt oev in
-      eliminate forall h_. exists lt_. steps e' e'' h_ lt_ with (h++lt_ev);
-      assert (exists lt_. steps e' e'' (h++lt_ev) lt_);
-      eliminate exists lt_. steps e' e'' (h++lt_ev) lt_
-      returns is_value e'' \/ indexed_can_step e'' (h'++lt') with _. begin
-        lem_step_implies_steps e e' h oev;
-        assert (steps e e' h lt_ev);
-        lem_steps_transitive e e' e'' h lt_ev lt_;
-        eliminate forall e' h lt. steps e e' h lt ==> (is_value e' \/ indexed_can_step e' (h++lt)) with e'' h (lt_ev @ lt_);
-        introduce indexed_can_step e'' (h++(lt_ev @ lt_)) ==> indexed_can_step e'' (h'++lt') with _. begin
-          indexed_can_step_history_independence e'' (h++(lt_ev @ lt_))
-        end
-      end)
-    end
-  end
-
-let indexed_irred_history_independence (e:closed_exp) (h:history) :
-  Lemma (requires indexed_irred e h)
-        (ensures forall h'. indexed_irred e h') =
-  introduce forall (h':history) (e':closed_exp) (oev':option (event_h h')). step e e' h' oev' ==> False with begin
-    introduce step e e' h' oev' ==> False with _. begin
-      bind_squash #(step e e' h' oev') () (fun st ->
-      step_history_independence st;
-      eliminate forall h_. exists oev_. step e e' h_ oev_ with h;
-      eliminate exists oev_. step e e' h oev_
-      returns False with _. begin
-        eliminate forall e_ oev_. step e e_ h oev_ ==> False with e' oev_
-      end)
-    end
-  end
-
-let sem_expr_shape_history_independence (e:closed_exp) (h:history) (t:typ) :
-  Lemma (requires indexed_sem_expr_shape t e h)
-        (ensures forall h'. indexed_sem_expr_shape t e h') =
-  introduce forall (h':history) (e':closed_exp) (lt':local_trace h'). steps e e' h' lt' /\ indexed_irred e' (h'++lt') ==> sem_value_shape t e' with begin
-    introduce steps e e' h' lt' /\ indexed_irred e' (h'++lt') ==> sem_value_shape t e' with _. begin
-      bind_squash #(steps e e' h' lt') () (fun sts ->
-      steps_history_independence sts;
-      eliminate forall h_. exists lt_. steps e e' h_ lt_ with h;
-      eliminate exists lt_. steps e e' h lt_
-      returns sem_value_shape t e' with _. begin
-        eliminate forall e_ (lt_:local_trace h). steps e e_ h lt_ /\ indexed_irred e_ (h++lt_) ==> sem_value_shape t e_ with e' lt_;
-        assert (steps e e' h lt_ /\ indexed_irred e' (h++lt_) ==> sem_value_shape t e');
-        indexed_irred_history_independence e' (h'++lt')
-      end)
-    end
-  end
-
-let lem_step_preserve_sem_expr_shape (e e':closed_exp) (h:history) (oev:option (event_h h)) (t:typ) :
-  Lemma
-    (requires indexed_sem_expr_shape t e h /\ step e e' h oev)
-    (ensures indexed_sem_expr_shape t e' (h++(as_lt oev))) =
-  introduce forall e'' lt'. steps e' e'' (h++(as_lt oev)) lt' /\ indexed_irred e'' ((h++(as_lt oev))++lt') ==> sem_value_shape t e'' with begin
-    introduce _  ==> sem_value_shape t e'' with _. begin
-      bind_squash #(steps e' e'' (h++(as_lt oev)) lt') () (fun sts ->
-      steps_history_independence sts;
-      let lt_ev = as_lt oev in
-      eliminate forall h_. exists lt_. steps e' e'' h_ lt_ with (h++lt_ev);
-      eliminate exists lt_. steps e' e'' (h++lt_ev) lt_
-      returns sem_value_shape t e'' with _. begin
-        lem_step_implies_steps e e' h oev;
-        lem_steps_transitive e e' e'' h lt_ev lt_;
-        eliminate forall e' lt. steps e e' h lt /\ indexed_irred e' (h++lt) ==> sem_value_shape t e' with e'' (lt_ev @ lt_);
-        indexed_irred_history_independence e'' ((h++(as_lt oev))++lt')
-      end)
-    end
-  end
-
-let indexed_irred_history_independence (e:closed_exp) (h:history) :
-  Lemma (requires indexed_irred e h)
-        (ensures forall h'. indexed_irred e h') =
-  introduce forall (h':history) (e':closed_exp) (oev':option (event_h h')). step e e' h' oev' ==> False with begin
-    introduce step e e' h' oev' ==> False with _. begin
-      bind_squash #(step e e' h' oev') () (fun st ->
-      step_history_independence st;
-      eliminate forall h_. exists oev_. step e e' h_ oev_ with h;
-      eliminate exists oev_. step e e' h oev_
-      returns False with _. begin
-        eliminate forall e_ oev_. step e e_ h oev_ ==> False with e' oev_
-      end)
-    end
-  end
-
-let sem_expr_shape_history_independence (e:closed_exp) (h:history) (t:typ) :
-  Lemma (requires indexed_sem_expr_shape t e h)
-        (ensures forall h'. indexed_sem_expr_shape t e h') =
-  introduce forall (h':history) (e':closed_exp) (lt':local_trace h'). steps e e' h' lt' /\ indexed_irred e' (h'++lt') ==> sem_value_shape t e' with begin
-    introduce steps e e' h' lt' /\ indexed_irred e' (h'++lt') ==> sem_value_shape t e' with _. begin
-      bind_squash #(steps e e' h' lt') () (fun sts ->
-      steps_history_independence sts;
-      eliminate forall h_. exists lt_. steps e e' h_ lt_ with h;
-      eliminate exists lt_. steps e e' h lt_
-      returns sem_value_shape t e' with _. begin
-        eliminate forall e_ (lt_:local_trace h). steps e e_ h lt_ /\ indexed_irred e_ (h++lt_) ==> sem_value_shape t e_ with e' lt_;
-        assert (steps e e' h lt_ /\ indexed_irred e' (h++lt_) ==> sem_value_shape t e');
-        indexed_irred_history_independence e' (h'++lt')
-      end)
-    end
-  end
-  *)
-
